WIP: Try to refactor the code with the new idea

Rsp.fst
@@ -9,137 +9,167 @@ open M4
 open Minterop
 open IO.Behavior
 
-noeq type language = {
-  interface : Type;
-
-  res : interface -> Type;
-  
-  prog: interface -> Type;
-  ctx : interface -> Type;
-  whole : interface -> Type;
-
-  link : (i:interface) -> ctx i -> prog i -> whole i;
-}
-
 noeq type compiler = {
-  source : language;
-  target : language;
-
-  cint : source.interface -> target.interface;
-
+  interface : Type;
   set_of_traces : Type -> Type;
-  beh_s : (i:source.interface) -> source.whole i -> set_of_traces (source.res i);
-  beh_t : (i:source.interface) -> target.whole (cint i) -> set_of_traces (target.res (cint i));
-  
-  included_in_s : (i:source.interface) -> set_of_traces (source.res i) -> set_of_traces (source.res i) -> Type;
-  included_in_t : (i:source.interface) -> set_of_traces (target.res (cint i)) -> set_of_traces (source.res i) -> Type;
+  monitorable_prop : Type;
+  safety_prop   : (#a:Type) -> monitorable_prop -> set_of_traces a;
 
-  rel_ctx : (i:source.interface) -> source.ctx i -> target.ctx (cint i) -> Type0;
+  res_s   : interface -> Type;
+  prog_s  : interface -> monitorable_prop -> Type;
+  ctx_s   : interface -> monitorable_prop -> Type;
+  whole_s : interface -> monitorable_prop -> Type;
+  link_s  : (#i:interface) -> (#pi:monitorable_prop) -> ctx_s i pi -> prog_s i pi -> Tot (whole_s i pi);
 
-  compile_prog : i:source.interface -> source.prog i -> target.prog (cint i);
-  compile_whole : i:source.interface -> source.whole i -> target.whole (cint i);
+  res_t   : interface -> Type;
+  prog_t  : interface -> monitorable_prop -> Type;
+  ctx_t   : interface -> Type;
+  whole_t : interface -> Type;
+  link_t  : (#i:interface) -> (#pi:monitorable_prop) -> ctx_t i -> prog_t i pi -> Tot (whole_t i);
+
+
+  beh_s : (#i:interface) -> (#pi:monitorable_prop) -> whole_s i pi -> set_of_traces (res_s i);
+  beh_t : (#i:interface) -> whole_t i -> set_of_traces (res_t i);
+
+  included_in_s : (#i:interface) -> set_of_traces (res_s i) -> set_of_traces (res_s i) -> Type;
+  included_in_t : (#i:interface) -> set_of_traces (res_t i) -> set_of_traces (res_s i) -> Type;
+
+  compile_prog  : (#i:interface) -> (#pi:monitorable_prop) -> prog_s i pi -> Tot (prog_t i pi);
+  compile_whole : (#i:interface) -> (#pi:monitorable_prop) -> whole_s i pi -> Tot (whole_t i);
 }
   
-let rsp (op:compiler) (i:op.source.interface) (ps:op.source.prog i) (pi_set:op.set_of_traces (op.source.res i)) : Type0 =
-  (forall cs. op.beh_s i (cs `op.source.link i` ps) `op.included_in_s i` pi_set)
-  ==> (forall (ct: op.target.ctx (op.cint i)). (
-      let pt = op.compile_prog i ps in
-      op.beh_t i (ct `op.target.link (op.cint i)` pt) `op.included_in_t i` pi_set))
+let rsp (op:compiler) (i:op.interface) (pi:op.monitorable_prop) (ps:op.prog_s i pi) : Type0 =
+  (forall cs. op.beh_s (cs `op.link_s` ps) `op.included_in_s` (op.safety_prop pi))
+  ==> (forall (ct: op.ctx_t i). (
+      let pt = op.compile_prog ps in
+      op.beh_t (ct `op.link_t` pt) `op.included_in_t` (op.safety_prop pi)))
 
-let tp (op:compiler) (i:op.source.interface) (ws:op.source.whole i) (pi_set:op.set_of_traces (op.source.res i)): Type0 =
-    ((op.beh_s i ws `op.included_in_s i` pi_set) ==>  (op.beh_t i (op.compile_whole i ws) `op.included_in_t i` pi_set))
-
-let ccc (op:compiler) (i:op.source.interface) (ps:op.source.prog i) (cs:op.source.ctx i) (ct:op.target.ctx (op.cint i)) : Type0 =
-  op.rel_ctx i cs ct ==> (
-  let pt : op.target.prog (op.cint i) = op.compile_prog i ps in
-  op.beh_t i (ct `op.target.link (op.cint i)` pt) `op.included_in_t i` 
-    (op.beh_s i (cs `op.source.link i` ps)))
-    
+let tp (op:compiler) (i:op.interface) (pi:op.monitorable_prop) (ws:op.whole_s i pi) : Type0 =
+    ((op.beh_s ws `op.included_in_s` (op.safety_prop pi)) ==>  
+      (op.beh_t (op.compile_whole ws) `op.included_in_t` (op.safety_prop pi)))
 
 noeq type interface = {
   a : Type;  ad : exportable a;
   b : Type;  bd : ml b;         // b has to be importable and exportable
   c : Type;  cd : exportable c;
+  post : a -> events_trace -> maybe (events_trace * b) -> events_trace -> Type; 
+  cpost : checkable4 post;
 }
 
-type whole_s (pi:check_type) (i:interface) = unit -> GIO i.c pi
+type whole_s (i:interface) (pi:check_type) = unit -> M4wp i.c pi (fun _ _ _ -> True)
 type whole_t (i:interface) = unit -> M4 i.cd.etype
 
-type ctx_s (pi:check_type) (i:interface) = i.a -> GIO i.b pi
+type ctx_s (i:interface) (pi:check_type) = (x:i.a) -> M4wp i.b pi (i.post x)
+type ctx_p (i:interface) (pi:check_type) = i.ad.etype -> M4wp i.b pi (fun _ _ _ -> True)
 type ctx_t (i:interface) = i.ad.etype -> M4 i.b
 
-type prog_s (pi:check_type) (i:interface) = ctx_s pi i -> GIO i.c pi
-type prog_t (i:interface) = ctx_t i -> M4 i.cd.etype
+type prog_s (i:interface) (pi:check_type) = ctx_s i pi -> M4wp i.c pi (fun _ _ _ -> True)
+type prog_t (i:interface) (pi:check_type) = ctx_p i pi -> M4 i.cd.etype
 
 unfold 
-let beh_s #a #b (pi:check_type) (ws:a -> GIO b pi) (x:a) =
+let beh_s 
+  #a
+  #b
+  (pi:check_type) 
+  (ws:(x:a -> M4wp b pi (fun _ _ _ -> True))) 
+  (x:a) =
   behavior (reify (ws x) (gio_post pi []) [])
 
 unfold
 let beh_t #a #b (wt:a -> M4 b) (x:a) =
   behavior (reify (wt x) (fun _ -> True))
 
-val import_ctx_t : (#pi:check_type) -> (#i:interface) -> ctx_t i -> option (ctx_s pi i)
-let import_ctx_t #pi #i f =
-  let f' : (ctx_s pi i) = (
-    fun (x:i.a) ->
-      let x : i.ad.etype = export x in
-      let tree = reify (f x) (fun r -> True) in
-      _import_M4_to_GIO #i.b tree pi <: GIO i.b pi) in 
-  Some f'
+let rec handle #t2 (tree : io (t2)) (pi:check_type) : M4wp t2 pi (fun _ _ _ -> True) = begin
+  match tree with
+  | Return r -> r 
+  | Throw r -> IOStHist.throw r
+  | Cont (Call cmd argz fnc) ->
+      let rez : res cmd = IOStHist.dynamic_cmd cmd pi argz in
+      FStar.WellFounded.axiom1 fnc (Inl rez);
+      let z' : sys io_cmds io_cmd_sig t2 = fnc (Inl rez) in
+      rev_append_rev_append ();
+      handle z' pi
+end
+
+let extract_local_events (s0 s1:events_trace) :
+  Pure events_trace
+    (requires (exists le. s1 == apply_changes s0 le))
+    (ensures (fun le -> s1 == apply_changes s0 le)) = 
+  admit ();
+  assert (List.length s1 >= List.length s0);
+  let n : nat = (List.length s1) - (List.length s0) in
+  let (le, _) = List.Tot.Base.splitAt n s1 in
+  List.rev le
+
+let ctx_p_to_ctx_s
+  (i  : interface)
+  (pi : check_type)
+  (cp  : ctx_p i pi) : 
+  Tot (ctx_s i pi) =
+  fun (x:i.a) -> 
+    admit ();
+    let s0 : events_trace = IOStHist.get () in
+    let result : i.b = cp x in
+    let s1 : events_trace = IOStHist.get () in
+    let le = extract_local_events s0 s1 in
+
+    if check4 #i.a #i.b #i.post #i.cpost x s0 (Inl (s1, result)) le then (
+      assert (i.post x s0 (Inl (s1, result)) le);
+      result
+    ) else IOStHist.throw Contract_failure
+
+let ctx_t_to_ctx_p
+  (i  : interface)
+  (pi : check_type)
+  (ct : ctx_t i) :
+  Tot (ctx_p i pi) =
+  fun (x:i.ad.etype) -> handle (reify (ct x) (fun _ -> True)) pi
 
 let export_prog_s
   (i  : interface)
   (pi : check_type)
-  (f  : prog_s pi i) : 
-  Tot (prog_t i) =
-    (fun (ct:ctx_t i) ->
-      let Some (cs : ctx_s pi i) = import_ctx_t ct in
+  (f  : prog_s i pi) : 
+  Tot (prog_t i pi) =
+    (fun (ct:ctx_p i pi) ->
+      let cs = ctx_p_to_ctx_s i pi ct in
       let tree : io (events_trace * i.c) = reify (f cs) (gio_post pi []) [] in
-      export (M4wp?.reflect (fun _ -> iost_to_io tree) <: M4wp i.c (fun p -> forall res. p res)))
+      export (MFOUR?.reflect (fun _ -> iost_to_io tree) <: MFOUR i.c (fun p -> forall res. p res)))
 
-let secure_interop (pi:check_type) : compiler = {
-  source = {
-    interface = interface;
-    res   = (fun i -> maybe (events_trace * i.c));
-    prog  = (fun i -> prog_s pi i);
-    ctx   = (fun i -> ctx_s pi i);
-    whole = (fun i -> whole_s pi i);
-  
-    link = (fun i c p -> (fun _ -> p c) <: whole_s pi i);
-  };
+let seci : compiler = {
+  interface = interface;
+  monitorable_prop = check_type;
+  safety_prop = pi_to_set;
 
-  target = {
-    interface = interface;
-    res   = (fun i -> maybe (i.cd.etype));
-    prog  = (fun i -> prog_t i);
-    ctx   = (fun i -> ctx_t i);
-    whole = (fun i -> whole_t i);
-  
-    link = (fun i c p -> (fun _ -> p c) <: whole_t i);
-  };
-
-  cint = (fun i -> i);
-  
   set_of_traces = set_of_traces;
 
-  beh_s = (fun i w -> beh_s #unit #i.c pi w ());
-  beh_t = (fun i w -> beh_t #unit #i.cd.etype w ());
+  res_s   = (fun i -> maybe (events_trace * i.c));
+  prog_s  = (fun i pi -> prog_s i pi);
+  ctx_s   = (fun i pi -> ctx_s i pi);
+  whole_s = (fun i pi -> whole_s i pi);
   
-  included_in_s = (fun i -> included_in id);
-  included_in_t = (fun i -> included_in #(maybe i.cd.etype) #(maybe (events_trace * i.c)) (inl_app (compose export cdr)));
+  link_s = (fun #i #pi c p -> (fun _ -> p c) <: whole_s i pi);
 
-  rel_ctx = (fun i cs ct -> let Some cs' = import_ctx_t #pi #i ct in cs' == cs);
+  res_t   = (fun i -> maybe (i.cd.etype));
+  prog_t  = (fun i pi -> prog_t i pi);
+  ctx_t   = (fun i -> ctx_t i);
+  whole_t = (fun i -> whole_t i);
+  link_t = (fun #i #pi c p -> (fun _ -> p (ctx_t_to_ctx_p i pi c)) <: whole_t i);
+
+  beh_s = (fun #i #pi w -> beh_s #unit #i.c pi w ());
+  beh_t = (fun #i w -> beh_t #unit #i.cd.etype w ());
   
-  compile_prog  = (fun i -> export_prog_s i pi);
-  compile_whole = (fun i -> _export_GIO_arrow_spec pi);
+  included_in_s = (fun #i -> included_in id);
+  included_in_t = (fun #i -> included_in #(maybe i.cd.etype) #(maybe (events_trace * i.c)) (inl_app (compose export cdr)));
+
+  compile_prog  = (fun #i #pi -> export_prog_s i pi);
+  compile_whole = (fun #i #pi -> _export_GIO_arrow_spec pi);
 }
 
-let _export_GIO_lemma
+let _export_whole_lemma
   #t1 {| d1:importable t1 |} 
   #t2 {| d2:exportable t2 |}
   (pi : check_type) 
-  (f:(x:t1 -> GIO t2 pi)) 
+  (f:(x:t1 -> M4wp t2 pi (fun _ _ _ -> True))) 
   (x':d1.itype) : 
   Lemma (
     let ef : d1.itype -> M4 d2.etype = _export_GIO_arrow_spec pi f in
@@ -153,9 +183,9 @@ let _export_GIO_lemma
   match import x' with
   | Some x -> begin
     let l = reify (ef x') (fun _ -> True) in
-    let __ll : unit -> M4wp d2.etype (fun p -> forall res. p res) = (fun _ -> 
+    let __ll : unit -> MFOUR d2.etype (fun p -> forall res. p res) = (fun _ -> 
             let tree : io (events_trace * t2) = reify (f x) (gio_post pi []) [] in
-            export (M4wp?.reflect (fun _ -> iost_to_io tree) <: M4wp t2 (fun p -> forall res. p res))) in
+            export (MFOUR?.reflect (fun _ -> iost_to_io tree) <: MFOUR t2 (fun p -> forall res. p res))) in
     let ll = reify (__ll ()) (fun _ -> True) in
     // TODO: Cezar: The idea behind this is to get rid of the `match`  
     // because we did it already in the proof.
@@ -174,7 +204,7 @@ let _export_GIO_lemma
         behavior ll;
         `included_in_id` {}
         behavior (reify (
-            (export (M4wp?.reflect (ref (iost_to_io (reify (f x) (gio_post pi []) []))) <: M4wp t2 (fun p -> forall res. p res)) <: d2.etype)) (fun _ -> True));
+            (export (MFOUR?.reflect (ref (iost_to_io (reify (f x) (gio_post pi []) []))) <: MFOUR t2 (fun p -> forall res. p res)) <: d2.etype)) (fun _ -> True));
         // TODO: Cezar: this should be just an unfolding of `reify`. I talked with Guido
         // and it seems using tactics is not a solution to unfold `reify` for 
         // layered effects because: "reification of layered effects is explicitly disabled
@@ -186,24 +216,24 @@ let _export_GIO_lemma
         `included_in_id` { admit () }
         // TODO: Cezar: is the 3rd argument correct? I suppose it should use pre and post
         behavior (M4.ibind t2 d2.etype (fun p -> forall res. p res) (fun x -> m4_return_wp (d2.etype) (export x))
-            (reify (M4wp?.reflect (ref (iost_to_io (reify (f x) (gio_post pi []) []))) <: M4wp t2 (fun p -> forall res. p res)))
-            (fun x -> lift_pure_m4wp d2.etype (fun p -> p (export x)) (fun _ -> export x)) (fun _ -> True));
+            (reify (MFOUR?.reflect (ref (iost_to_io (reify (f x) (gio_post pi []) []))) <: MFOUR t2 (fun p -> forall res. p res)))
+            (fun x -> lift_pure_mfour d2.etype (fun p -> p (export x)) (fun _ -> export x)) (fun _ -> True));
     };
 
     beh_included_bind_tot #t2 #d2.etype
-        (reify (M4wp?.reflect (ref (iost_to_io (reify (f x) (gio_post pi []) []))) <: M4wp t2 (fun p -> forall res. p res)) (compute_post t2 (Mkexportable?.etype d2) (fun x -> m4_return_wp (Mkexportable?.etype d2) (export x)) (fun _ -> True)))
+        (reify (MFOUR?.reflect (ref (iost_to_io (reify (f x) (gio_post pi []) []))) <: MFOUR t2 (fun p -> forall res. p res)) (compute_post t2 (Mkexportable?.etype d2) (fun x -> m4_return_wp (Mkexportable?.etype d2) (export x)) (fun _ -> True)))
         export;
 
     assert (
         (behavior (M4.ibind t2 d2.etype (fun p -> forall res. p res) (fun x -> m4_return_wp (d2.etype) (export x))
-            (reify (M4wp?.reflect (ref (iost_to_io (reify (f x) (gio_post pi []) []))) <: M4wp t2 (fun p -> forall res. p res)))
-            (fun x -> lift_pure_m4wp d2.etype (fun p -> p (export x)) (fun _ -> export x)) (fun _ -> True)))
+            (reify (MFOUR?.reflect (ref (iost_to_io (reify (f x) (gio_post pi []) []))) <: MFOUR t2 (fun p -> forall res. p res)))
+            (fun x -> lift_pure_mfour d2.etype (fun p -> p (export x)) (fun _ -> export x)) (fun _ -> True)))
         `included_in (inl_app export)`
-        (behavior (reify (M4wp?.reflect (ref (iost_to_io (reify (f x) (gio_post pi []) []))) <: M4wp t2 (fun p -> forall res. p res)) (fun _ -> True)))
+        (behavior (reify (MFOUR?.reflect (ref (iost_to_io (reify (f x) (gio_post pi []) []))) <: MFOUR t2 (fun p -> forall res. p res)) (fun _ -> True)))
     ) by (unfold_def (`ibind));
 
     calc (included_in_id) {
-        behavior (reify (M4wp?.reflect (ref (iost_to_io (reify (f x) (gio_post pi []) []))) <: M4wp t2 (fun p -> forall res. p res)) (fun _ -> True));
+        behavior (reify (MFOUR?.reflect (ref (iost_to_io (reify (f x) (gio_post pi []) []))) <: MFOUR t2 (fun p -> forall res. p res)) (fun _ -> True));
         `included_in_id` {}
         behavior (iost_to_io (reify (f x) (gio_post pi []) []));
     };
@@ -229,143 +259,155 @@ let _export_GIO_lemma
     }
   end
 
-let export_GIO_lemma 
+let export_whole_lemma 
   #t1 {| d1:importable t1 |} 
   #t2 {| d2:exportable t2 |}
   (pi:check_type)
-  (f:(x:t1 -> GIO t2 pi)) : 
+  (f:(x:t1 -> M4wp t2 pi (fun _ _ _ -> True))) : 
   Lemma (forall (x':d1.itype). (
     let ef : d1.itype -> M4 d2.etype = export f in
     match import x' with
     | Some x -> (
         beh_t ef x' `included_in (inl_app (compose export cdr))` beh_s pi f x)
     | None ->  beh_t ef x' `included_in id` empty_set ())) =
-  Classical.forall_intro (_export_GIO_lemma pi f)
+  admit ();
+  Classical.forall_intro (_export_whole_lemma pi f)
 
-let beh_export_unit_GIO_lemma
+let beh_export_unit_whole_lemma
   #t2 {| d2:exportable t2 |}
   (pi:check_type)
-  (f:(unit -> GIO t2 pi)) : 
+  (f:(unit -> M4wp t2 pi (fun _ _ _ -> True))) : 
   Lemma (
     let ef : unit -> M4 d2.etype = _export_GIO_arrow_spec pi f in
     beh_t ef () `included_in (inl_app (compose export cdr))` beh_s pi f ()) =
-  _export_GIO_lemma pi f ()
+  _export_whole_lemma pi f ()
 
-  
-let rsp_premise
-  (i:interface)
-  (pi : check_type)
-  (ps : prog_s pi i)
-  (ct : ctx_t i) :
-  Lemma (
-    let Some (cs : ctx_s pi i) = import_ctx_t ct in
-    beh_s pi ps cs `included_in id` (pi_to_set pi)) =
-  let Some (cs : ctx_s pi i) = import_ctx_t ct in
-  beh_gio_in_pi (ctx_s pi i) i.c pi ps cs
+val import_ctx_t : (#i:interface) -> (#pi:check_type) -> ctx_t i -> ctx_s i pi
+let import_ctx_t #i #pi ct =
+  ctx_p_to_ctx_s i pi (
+    ctx_t_to_ctx_p i pi ct)
 
 let beh_export_ps_ct_in_export_ws
   (i  : interface)
   (pi : check_type)
-  (ps : prog_s pi i)
-  (ct : ctx_t i) : 
+  (ps : prog_s i pi)
+  (cp : ctx_p i pi) : 
   Lemma (
-    let Some (cs : ctx_s pi i) = import_ctx_t ct in
-    let ws : unit -> GIO i.c pi = fun _ -> ps cs in
-    let pt : (ctx_t i) -> M4 i.cd.etype = export_prog_s i pi ps in
-    let wt : unit -> M4 i.cd.etype = _export_GIO_arrow_spec pi ws in
-    beh_t pt ct `included_in id` beh_t wt ()
+    let (cs : ctx_s i pi) = ctx_p_to_ctx_s i pi cp in
+    let ws : whole_s i pi = fun _ -> ps cs in
+    let pt : prog_t i pi = export_prog_s i pi ps in
+    let wt : whole_t i = _export_GIO_arrow_spec pi ws in
+    beh_t pt cp `included_in id` beh_t wt ()
   ) = 
-  let Some (cs : ctx_s pi i) = import_ctx_t ct in
-  let ws : whole_s pi i = fun _ -> ps cs in
-  let pt : (ctx_t i) -> M4 i.cd.etype = export_prog_s i pi ps in
+  let (cs : ctx_s i pi) = ctx_p_to_ctx_s i pi cp in
+  let ws : whole_s i pi = fun _ -> ps cs in
+  let pt : prog_t i pi = export_prog_s i pi ps in
   let wt : whole_t i = _export_GIO_arrow_spec pi ws in
   
   let included_in_id #a = included_in #a #a (id #a) in
-  assert (import () == Some ());
+  // assert (import () == Some ());
   // TODO: apply l_to_r for: import () == Some ()
   //       apply l_to_r for: import_ctx_t ct == Some b
   //       Qed.
   // Related github issue: https://github.com/FStarLang/FStar/issues/2169
-  assert (reify (pt ct) (fun _ -> True) == reify (wt ()) (fun _ -> True)) by (
+  assert (reify (pt cp) (fun _ -> True) == reify (wt ()) (fun _ -> True)) by (
     unfold_def (`export_prog_s);
-    unfold_def (`_export_GIO_arrow_spec);
+    unfold_def (`_export_GIO_arrow_spec)
     // dump "x"
-    tadmit ()
+    // tadmit ()
   )
-    
-let rsp_conclusion 
-  (i  : interface)
-  (pi : check_type)
-  (ps : prog_s pi i)
-  (ct : ctx_t i) :
+
+let seci_rsp_0
+  (i   : seci.interface)
+  (pi  : seci.monitorable_prop)
+  (ps  : seci.prog_s i pi)
+  (ct  : seci.ctx_t i) :
   Lemma (
-    let pt : prog_t i = export_prog_s i pi ps in
-    beh_t pt ct `included_in #_ #(maybe (events_trace * i.c)) (inl_app (compose export cdr))` (pi_to_set pi)) = 
-  let Some (cs : ctx_s pi i) = import_ctx_t ct in
-  let ws : whole_s pi i = fun _ -> ps cs in
-  beh_gio_in_pi unit i.c pi ws (); // Beh (ws ()) in pi
-  beh_export_unit_GIO_lemma #i.c #i.cd pi ws; // Beh (export ws ()) in Beh (ws ())
-  beh_export_ps_ct_in_export_ws i pi ps ct // Beh ((export ps) ct) in Beh (export ws ())
-
-let rsp_variant
-  (i  : interface)
-  (pi : check_type)
-  (ps : prog_s pi i)
-  (ct : ctx_t i) :
-  Lemma(
-    (forall (cs:(ctx_s pi i)). beh_s pi ps cs `included_in id` (pi_to_set pi)) 
-    ==> 
-    (let pt : prog_t i = export_prog_s i pi ps in
-     beh_t pt ct `included_in #_ #(maybe (events_trace * i.c)) (inl_app (compose export cdr))` (pi_to_set pi))) = 
-  rsp_conclusion i pi ps ct
-
-
-let si = secure_interop
-
-// This was working before, but after parameterizing with the interface
-// some types do not match and some manual needs to be done to show that b and b' are the same or 
-// smth. 
-let rsp_simple_linking''
-  (pi  : check_type)
-  (i   : (si pi).source.interface)
-  (ps  : (si pi).source.prog i)
-  (ct  : (si pi).target.ctx ((si pi).cint i)) 
-  pi_set :
-  Lemma (
-  (forall cs. (si pi).beh_s i (cs `(si pi).source.link i` ps) `(si pi).included_in_s i` pi_set)
+  (forall (cs:seci.ctx_s i pi). 
+    (seci.beh_s #i #pi (cs `seci.link_s #i #pi` ps)) `seci.included_in_s #i` (seci.safety_prop pi))
   ==>  (
-      let pt = (si pi).compile_prog i ps in
-      (si pi).beh_t i (ct `(si pi).target.link ((si pi).cint i)` pt) `(si pi).included_in_t i` pi_set)) = admit ();
-  let Some (cs:ctx_s pi i) = import_ctx_t ct in
-  let ws : whole_s pi i = fun _ -> ps cs in
-  assert (beh_s pi ws () `included_in id` beh_s pi ps cs);
-  beh_export_unit_GIO_lemma #i.c #i.cd pi ws; // Beh (export ws ()) in Beh (ws ())
-  beh_export_ps_ct_in_export_ws i pi ps ct // Beh ((export ps) ct) in Beh (export ws ())
- 
-let rsp_lemma
-  (pi : check_type)
-  (i  : (si pi).source.interface)
-  (ps : (si pi).source.prog i) :
-  Lemma (forall pi_set. rsp (secure_interop pi) i ps pi_set) =
-    Classical.forall_intro_2 (rsp_simple_linking'' pi i ps)
-  
-let tp_lemma
-  (pi : check_type)
-  (i : (si pi).source.interface)
-  (ws : (si pi).source.whole i) : 
-  Lemma (forall pi_set. tp (si pi) (i) (ws) pi_set)  = 
-  beh_export_unit_GIO_lemma #i.c #i.cd pi ws
+      let pt = seci.compile_prog #i ps in
+      seci.beh_t #i (ct `seci.link_t #i #pi` pt) `seci.included_in_t #i` (seci.safety_prop pi))) =
+  admit ();
+  let (cp:ctx_p i pi) = ctx_t_to_ctx_p i pi ct in
+  let (cs:seci.ctx_s i pi) = ctx_p_to_ctx_s i pi cp in
+  let ws : seci.whole_s i pi = seci.link_s #i #pi cs ps in
+  assert (seci.beh_s #i #pi ws `seci.included_in_s #i` (seci.safety_prop pi));
+  beh_export_unit_whole_lemma #i.c #i.cd pi ws; // Beh (export ws ()) in Beh (ws ())
+  beh_export_ps_ct_in_export_ws i pi ps cp // Beh ((export ps) ct) in Beh (export ws ())
 
-let secure_linker_respects_rsp () : 
-  Lemma (forall pi i ps pi_set. rsp (secure_interop pi) i ps pi_set)
-  by (
-    unfold_def(`rsp);
-    explode ();
-    rewrite_lemma 2 3;
-    norm [iota]
-  ) =
-  Classical.forall_intro_3 (rsp_lemma)
+let seci_rsp
+  (i  : seci.interface)
+  (pi : seci.monitorable_prop)
+  (ps : seci.prog_s i pi) :
+  Lemma (rsp seci i pi ps) =
+    Classical.forall_intro (seci_rsp_0 i pi ps)
   
-let secure_linker_respects_tp () :
-  Lemma (forall pi i ws pi_set. tp (si pi) i ws pi_set) = 
-    Classical.forall_intro_3 tp_lemma
+
+// let rsp_premise
+//   (i:interface)
+//   (pi : check_type)
+//   (ps : prog_s i pi)
+//   (ct : ctx_t i) :
+//   Lemma (
+//     let (cs : ctx_s i pi) = import_ctx_t ct in
+//     beh_s pi ps cs `included_in id` (pi_to_set pi)) =
+//   let (cs : ctx_s i pi) = import_ctx_t ct in
+//   beh_gio_in_pi (ctx_s i pi) i.c pi ps cs
+    
+// let rsp_conclusion 
+//   (i  : interface)
+//   (pi : check_type)
+//   (ps : prog_s pi i)
+//   (ct : ctx_t i) :
+//   Lemma (
+//     let pt : prog_t i = export_prog_s i pi ps in
+//     beh_t pt ct `included_in #_ #(maybe (events_trace * i.c)) (inl_app (compose export cdr))` (pi_to_set pi)) = 
+//   let Some (cs : ctx_s pi i) = import_ctx_t ct in
+//   let ws : whole_s pi i = fun _ -> ps cs in
+//   beh_gio_in_pi unit i.c pi ws (); // Beh (ws ()) in pi
+//   beh_export_unit_GIO_lemma #i.c #i.cd pi ws; // Beh (export ws ()) in Beh (ws ())
+//   beh_export_ps_ct_in_export_ws i pi ps ct // Beh ((export ps) ct) in Beh (export ws ())
+
+// let rsp_variant
+//   (i  : interface)
+//   (pi : check_type)
+//   (ps : prog_s pi i)
+//   (ct : ctx_t i) :
+//   Lemma(
+//     (forall (cs:(ctx_s pi i)). beh_s pi ps cs `included_in id` (pi_to_set pi)) 
+//     ==> 
+//     (let pt : prog_t i = export_prog_s i pi ps in
+//      beh_t pt ct `included_in #_ #(maybe (events_trace * i.c)) (inl_app (compose export cdr))` (pi_to_set pi))) = 
+//   rsp_conclusion i pi ps ct
+
+
+// let si = secure_interop
+ 
+// let rsp_lemma
+//   (pi : check_type)
+//   (i  : (si pi).source.interface)
+//   (ps : (si pi).source.prog i) :
+//   Lemma (forall pi_set. rsp (secure_interop pi) i ps pi_set) =
+//     Classical.forall_intro_2 (rsp_simple_linking'' pi i ps)
+  
+// let tp_lemma
+//   (pi : check_type)
+//   (i : (si pi).source.interface)
+//   (ws : (si pi).source.whole i) : 
+//   Lemma (forall pi_set. tp (si pi) (i) (ws) pi_set)  = 
+//   beh_export_unit_GIO_lemma #i.c #i.cd pi ws
+
+// let secure_linker_respects_rsp () : 
+//   Lemma (forall pi i ps pi_set. rsp (secure_interop pi) i ps pi_set)
+//   by (
+//     unfold_def(`rsp);
+//     explode ();
+//     rewrite_lemma 2 3;
+//     norm [iota]
+//   ) =
+//   Classical.forall_intro_3 (rsp_lemma)
+  
+// let secure_linker_respects_tp () :
+//   Lemma (forall pi i ws pi_set. tp (si pi) i ws pi_set) = 
+//     Classical.forall_intro_3 tp_lemma
